HoareLogic/OperationalSemanticsGenerator.v
@@ -7,6 +7,7 @@ Require Import Logic.lib.Coqlib.
 Require Import Logic.lib.NatChoice.
 Require Import Logic.lib.Stream.SigStream.
 Require Import Logic.lib.Stream.StreamFunctions.
+Require Import Logic.lib.Stream.StreamSplit.
 Require Import Logic.MinimunLogic.LogicBase.
 Require Import Logic.PropositionalLogic.KripkeSemantics.
 Require Import Logic.SeparationLogic.SeparationAlgebra.
@@ -18,6 +19,8 @@ Require Import Logic.HoareLogic.SmallStepSemantics.
 Require Import Logic.HoareLogic.LocalTraceSemantics.
 Require Import Logic.HoareLogic.BigStepSemantics.
 
+Module SSS_SimpleSSS.
+
 Instance SSS_SimpleSSS
          {P: ProgrammingLanguage}
          {state: Type}
@@ -25,6 +28,10 @@ Instance SSS_SimpleSSS
          (final_state: cmd * state -> Prop):
   SmallStepSemantics P state :=
   Build_SmallStepSemantics _ _ (SimpleSmallStepSemantics.step final_state).
+
+End SSS_SimpleSSS.
+
+Module LTS_SSS.
 
 Instance LTS_SSS
          {P: ProgrammingLanguage}
@@ -134,6 +141,7 @@ Proof.
   + intros.
     destruct H as [? ? _ _ _ _ _ ?].
     hnf; intros.
+    unfold ctrace2trace in tr_ctr.
     rewrite tr_ctr, stream_map_spec in H, H0.
     specialize (ctr_sequential k).
     destruct (ctr k) as [[[c0 s0] mcs] |]; [| congruence].
@@ -143,6 +151,254 @@ Proof.
     specialize (ctr_sequential _ _ _ _ eq_refl eq_refl).
     subst mcs; auto.
 Defined.
+
+Lemma trace_split2
+        {P: ProgrammingLanguage}
+        {iP: ImperativeProgrammingLanguage P}
+        {state: Type}:
+  forall R (ctr: trace (cmd * state)) c c' s mcs,
+    sequential_trace ctr ->
+    sound_trace R ctr ->
+    begin_end_state (c, s) ctr mcs ->
+    (exists ctr1 ctr2 s',
+       sequential_trace ctr1 /\
+       sound_trace R ctr1 /\
+       begin_end_state (c, s) ctr1 (Terminating (c', s')) /\
+       sound_trace (fun cs _ => fst cs <> c') ctr1 /\
+       sequential_trace ctr2 /\
+       sound_trace R ctr2 /\
+       begin_end_state (c', s') ctr2 mcs /\
+       ctr = stream_app ctr1 ctr2) \/
+    sound_trace (fun cs _ => fst cs <> c') ctr.
+Proof.
+  intros.
+  destruct (cut2_exists ctr (fun csmcs => fst (fst csmcs) = c')).
+  + destruct H2 as [ctr1 [ctr2 [? [? [? [[[c0 s'] mcs0] [? ?]]]]]]].
+    left; exists ctr1, ctr2, s'.
+    simpl in H6; subst c0 ctr.
+    split; [| split; [| split; [| split; [| split; [| split; [| split]]]]]].
+    - apply trace_app_sequential1 in H; auto.
+    - apply trace_app_sound1 in H0; auto.
+    - admit.
+    - hnf; intros.
+      exact (H4 k _ H3).
+    - apply trace_app_sequential2 in H; auto.
+    - apply trace_app_sound2 in H0; auto.
+    - admit.
+    - auto.
+  + right.
+    hnf; intros.
+    exact (H2 k _ H3).
+Admitted.
+
+Lemma trace_split_head
+        {P: ProgrammingLanguage}
+        {iP: ImperativeProgrammingLanguage P}
+        {state: Type}:
+  forall R (ctr: trace (cmd * state)) c s mcs,
+    sequential_trace ctr ->
+    sound_trace R ctr ->
+    begin_end_state (c, s) ctr mcs ->
+    exists mcs',
+    R (c, s) mcs' /\
+    match mcs' with
+    | Terminating (c', s') => 
+       exists ctr',
+       sequential_trace ctr' /\
+       sound_trace R ctr' /\
+       begin_end_state (c', s') ctr' mcs /\
+       ctr = stream_app (singleton_trace (c, s) mcs') ctr'
+    | _ => ctr = singleton_trace (c, s) mcs'
+    end.
+Admitted.
+
+Module Partial.
+
+Export SmallStepSemantics.Partial.
+Export LocalTraceSemantics.Partial.
+Export BigStepSemantics.Partial.
+
+Lemma Ssequence_fin_left {P: ProgrammingLanguage} {iP: ImperativeProgrammingLanguage P} {niP: NormalImperativeProgrammingLanguage P} {state: Type} {kiM: KripkeIntuitionisticModel state} {SSS: SmallStepSemantics P state} {iSSS: ImpSmallStepSemantics P state SSS}:
+  forall (ctr: trace (cmd * state)) c c0 s1 cs,
+    sequential_trace ctr ->
+    sound_trace step ctr ->
+    sound_trace (fun cs _ => fst cs <> Ssequence Sskip c) ctr ->
+    begin_end_state (Ssequence c0 c, s1) ctr (lift_function (pair (Ssequence Sskip c)) cs) ->
+    exists ctr',
+      sequential_trace ctr' /\
+      sound_trace step ctr' /\
+      begin_end_state (c0, s1) ctr' (lift_function (pair Sskip) cs) /\
+      ctrace2trace ctr' = ctrace2trace ctr.
+Admitted.
+
+Lemma Ssequence_progress_left {P: ProgrammingLanguage} {iP: ImperativeProgrammingLanguage P} {niP: NormalImperativeProgrammingLanguage P} {state: Type} {kiM: KripkeIntuitionisticModel state} {SSS: SmallStepSemantics P state} {iSSS: ImpSmallStepSemantics P state SSS}:
+  forall (ctr: trace (cmd * state)) c c0 s1 mcs,
+    sequential_trace ctr ->
+    sound_trace step ctr ->
+    sound_trace (fun cs _ => fst cs <> Ssequence Sskip c) ctr ->
+    begin_end_state (Ssequence c0 c, s1) ctr mcs ->
+    (exists c2 s2, mcs = Terminating (Ssequence c2 c, s2)) \/
+    mcs = NonTerminating \/ mcs = Error.
+Admitted.
+
+Instance iLTS_SSS {P: ProgrammingLanguage} {iP: ImperativeProgrammingLanguage P} {niP: NormalImperativeProgrammingLanguage P} {state: Type} {kiM: KripkeIntuitionisticModel state} (SSS: SmallStepSemantics P state) {iSSS: ImpSmallStepSemantics P state SSS}: ImpLocalTraceSemantics P state (LTS_SSS SSS).
+Proof.
+  refine (Build_ImpLocalTraceSemantics _ _ _ _ _ _ SmallStepSemantics.Partial.eval_bool_stable _ _ _ _).
+  + intros.
+    destruct H as [ctr _ ? ? mcs' ? _ ?].
+    inversion ctr_begin_end_state.
+    - subst.
+      unfold ctrace2trace.
+      rewrite stream_map_empty_stream.
+      apply empty_stream_is_empty.
+    - rename ms into mcs.
+      subst.
+      exfalso.
+      pose proof ctr_sound 0 (Sskip, s) mcs H0.
+      rewrite step_Sskip in H2; auto.
+    - rename ms into mcs.
+      subst.
+      exfalso.
+      pose proof ctr_sound 0 (Sskip, s) mcs H0.
+      rewrite step_Sskip in H1; auto.
+  + intros.
+    destruct H.
+    destruct (trace_split2 step ctr _ (Ssequence Sskip c2) _ _ ctr_sequential ctr_sound ctr_begin_end_state).
+    - destruct H as [ctr1 [ctrd2 [s' [? [? [? [? [? [? [? ?]]]]]]]]]].
+      left; exists (ctrace2trace ctr1), (ctrace2trace ctrd2).
+      subst ctr.
+      split; [| split]; [| | auto].
+      * destruct (Ssequence_fin_left _ _ _ _ (Terminating s') H H0 H2 H1) as [ctr1' [? [? [? ?]]]].
+        apply (SmallStepSemantics.Build_denote _ _ _ _ _ ctr1' H6 H7 _ _ H8).
+       ++ simpl; intros; rewrite step_Sskip; auto.
+       ++ symmetry; auto.
+      * destruct (trace_split_head step ctrd2 _ _ _ H3 H4 H5) as [cs [? ?]].
+        apply step_Ssequence in H6.
+        destruct H6;
+          [| destruct H6 as [? [? ?]]; rewrite step_Sskip in H6; tauto].
+        destruct H6 as [ms [_ [? ?]]].
+        subst cs; destruct ms; simpl in H7.
+       ++ right.
+          exists (singleton_trace s' Error).
+          split; [| split].
+         -- apply singleton_trace_decrease; auto.
+         -- right; exists s'.
+            apply begin_end_state_singleton_trace.
+         -- subst.
+            stream_extensionality k; destruct k as [| [| ]]; auto.
+       ++ right.
+          exists (singleton_trace s' NonTerminating).
+          split; [| split].
+         -- apply singleton_trace_decrease; auto.
+         -- left; exists s'.
+            apply begin_end_state_singleton_trace.
+         -- subst.
+            stream_extensionality k; destruct k as [| [| ]]; auto.
+       ++ destruct H7 as [ctr2 [? [? [? ?]]]].
+          left; exists (singleton_trace s' (Terminating s0)), (ctrace2trace ctr2).
+          subst ctrd2.
+          split; [| split].
+         -- apply singleton_trace_decrease; auto.
+         -- apply (SmallStepSemantics.Build_denote _ _ _ _ _ ctr2 H7 H8 _ _ H9); auto.
+         -- unfold ctrace2trace.
+            rewrite stream_map_stream_app.
+            f_equal.
+            stream_extensionality k; destruct k as [| [| ]]; auto.
+      * subst tr.
+        unfold ctrace2trace.
+        rewrite stream_map_stream_app.
+        reflexivity.
+    - right.
+      exists tr.
+      assert (mcs = NonTerminating \/ mcs = Error).
+      Focus 1. {
+        destruct (Ssequence_progress_left ctr _ _ _ _
+                   ctr_sequential ctr_sound H ctr_begin_end_state);
+          [exfalso | auto].
+        destruct H0 as [?c [?s ?]].
+        subst mcs.
+        pose proof step_defined (Ssequence c c2) s0 (Ssequence_Sskip _ _).
+        clear - end_state_valid H0; firstorder.
+      } Unfocus.
+      split; [| split]; auto.
+      * set (cs := lift_function snd mcs).
+        assert (mcs = lift_function (pair (Ssequence Sskip c2)) cs) by (destruct H0; subst; auto).
+        rewrite H1 in ctr_begin_end_state.
+        destruct (Ssequence_fin_left _ _ _ _ _ ctr_sequential ctr_sound H ctr_begin_end_state) as [ctr' [? [? [? ?]]]].
+        apply (SmallStepSemantics.Build_denote _ _ _ _ _ ctr' H2 H3 _ _ H4).
+       ++ clear H1; destruct H0; subst; simpl; auto.
+       ++ congruence.
+      * destruct H0; [left | right]; subst; exists s;
+        apply begin_end_state_ctrace in ctr_begin_end_state; auto.
+  + intros.
+    destruct H.
+    destruct (trace_split_head step ctr _ _ _ ctr_sequential ctr_sound ctr_begin_end_state) as [cs [? ?]].
+    apply step_Sifthenelse in H.
+    destruct H as [[? ?] | [? ?]]; [left | right];
+    destruct H1 as [ms [? ?]]; subst cs.
+    - destruct ms; [right | right | left].
+      * exists (singleton_trace s Error).
+        split; [| split].
+       ++ apply singleton_trace_decrease_test; auto.
+       ++ right; exists s.
+          apply begin_end_state_singleton_trace.
+       ++ simpl in H0.
+          subst.
+          stream_extensionality k; destruct k as [| [| ]]; auto.
+      * exists (singleton_trace s NonTerminating).
+        split; [| split].
+       ++ apply singleton_trace_decrease_test; auto.
+       ++ left; exists s.
+          apply begin_end_state_singleton_trace.
+       ++ simpl in H0.
+          subst.
+          stream_extensionality k; destruct k as [| [| ]]; auto.
+      * simpl in H0.
+        destruct H0 as [ctr' [? [? [? ?]]]].
+        exists (singleton_trace s (Terminating s0)), (ctrace2trace ctr').
+        split; [| split].
+       ++ apply singleton_trace_decrease_test; auto.
+       ++ apply (SmallStepSemantics.Build_denote _ _ _ _ _ ctr' H0 H2 _ _ H3); auto.
+       ++ subst.
+          unfold ctrace2trace.
+          rewrite stream_map_stream_app.
+          f_equal.
+          stream_extensionality k; destruct k as [| [| ]]; auto.
+    - destruct ms; [right | right | left].
+      * exists (singleton_trace s Error).
+        split; [| split].
+       ++ apply singleton_trace_decrease_test; auto.
+       ++ right; exists s.
+          apply begin_end_state_singleton_trace.
+       ++ simpl in H0.
+          subst.
+          stream_extensionality k; destruct k as [| [| ]]; auto.
+      * exists (singleton_trace s NonTerminating).
+        split; [| split].
+       ++ apply singleton_trace_decrease_test; auto.
+       ++ left; exists s.
+          apply begin_end_state_singleton_trace.
+       ++ simpl in H0.
+          subst.
+          stream_extensionality k; destruct k as [| [| ]]; auto.
+      * simpl in H0.
+        destruct H0 as [ctr' [? [? [? ?]]]].
+        exists (singleton_trace s (Terminating s0)), (ctrace2trace ctr').
+        split; [| split].
+       ++ apply singleton_trace_decrease_test; auto.
+       ++ apply (SmallStepSemantics.Build_denote _ _ _ _ _ ctr' H0 H2 _ _ H3); auto.
+       ++ subst.
+          unfold ctrace2trace.
+          rewrite stream_map_stream_app.
+          f_equal.
+          stream_extensionality k; destruct k as [| [| ]]; auto.
+  + 
+Abort.
+
+End Partial.
+End LTS_SSS.
+
+Module BSS_LTS.
 
 Instance BSS_LTS
          {P: ProgrammingLanguage}
@@ -158,32 +414,4 @@ Proof.
   auto.
 Defined.
 
-Module Partial.
-
-Export SmallStepSemantics.Partial.
-Export LocalTraceSemantics.Partial.
-Export BigStepSemantics.Partial.
-
-Instance iLTS_SSS {P: ProgrammingLanguage} {iP: ImperativeProgrammingLanguage P} {niP: NormalImperativeProgrammingLanguage P} {state: Type} {kiM: KripkeIntuitionisticModel state} (SSS: SmallStepSemantics P state) {iSSS: ImpSmallStepSemantics P state SSS}: ImpLocalTraceSemantics P state (LTS_SSS SSS).
-Proof.
-  refine (Build_ImpLocalTraceSemantics _ _ _ _ _ _ eval_bool_stable _ _ _ _).
-  + intros.
-    destruct H as [ctr _ ? ? mcs' ? _ ?].
-    inversion ctr_begin_end_state.
-    - subst.
-      rewrite stream_map_empty_stream.
-      apply empty_stream_is_empty.
-    - rename ms into mcs.
-      subst.
-      exfalso.
-      pose proof ctr_sound 0 (Sskip, s) mcs H0.
-      rewrite step_Sskip in H2; auto.
-    - rename ms into mcs.
-      subst.
-      exfalso.
-      pose proof ctr_sound 0 (Sskip, s) mcs H0.
-      rewrite step_Sskip in H1; auto.
-  + intros.
-Abort.
-
-End Partial.
+End BSS_LTS.
